very simple, unverified demo for rtac.

theories/RTac/CoreSimple.v
@@ -10,6 +10,10 @@ Require Import MirrorCore.SymI.
 Require Import MirrorCore.ExprI.
 Require Import MirrorCore.TypesI.
 Require Import MirrorCore.SubstI.
+Require Import MirrorCore.ExprDAs.
+Require Import MirrorCore.STac.Core.
+
+Require Import MirrorCore.Util.Forwardy.
 
 Set Implicit Arguments.
 Set Strict Implicit.
@@ -58,6 +62,9 @@ Section parameterized.
   Variable Subst_subst : Subst subst expr.
   Variable SubstOk_subst : @SubstOk _ _ _ _ Expr_expr Subst_subst.
 
+  Let propD := @exprD'_typ0 _ _ _ _ Prop _.
+
+(*
   Definition propD (tus tvs : list typ) (goal : expr) : ResType tus tvs Prop :=
     match exprD' tus tvs goal (@typ0 _ _ _ _) return ResType tus tvs Prop with
       | None => None
@@ -66,6 +73,7 @@ Section parameterized.
                | eq_refl => val
              end
     end.
+*)
 
   Fixpoint _foralls (ls : list typ)
   : (HList.hlist (typD nil) ls -> Prop) -> Prop :=
@@ -87,6 +95,14 @@ Section parameterized.
     match ls with
       | nil => P
       | l :: ls => l -> _impls ls P
+    end.
+
+  Fixpoint WellFormed_goal (goal : Goal) : Prop :=
+    match goal with
+      | GAlls _ goal'
+      | GExs _ goal'
+      | GHyps _ goal' => WellFormed_goal goal'
+      | GGoal s _ => WellFormed_subst s
     end.
 
   (** NOTE:
@@ -135,9 +151,14 @@ Section parameterized.
         end
     end.
 
+  (** The worry is that this isn't going to be strong enough,
+   ** especially when it comes to substitutions.
+   **)
   Definition rtac_sound tus tvs (tac : rtac) : Prop :=
     forall g g',
       tac g = Some g' ->
+      WellFormed_goal g ->
+      WellFormed_goal g' /\
       match goalD tus tvs g
           , goalD tus tvs g'
       with
@@ -182,11 +203,14 @@ Section parameterized.
     unfold THEN.
     intros.
     red. intros.
-    Require Import MirrorCore.Util.Forwardy.
-    forwardy.
-    eapply H in H1.
-    eapply H0 in H2.
-    forward. intuition.
+    forward.
+    eapply H in H1; clear H.
+    eapply H1 in H2; clear H1.
+    destruct H2.
+    eapply H0 in H3; eauto.
+    specialize (H3 H). forward_reason.
+    split; auto.
+    forward. eauto.
   Qed.
 
   Definition TRY (tac : rtac) : rtac :=
@@ -202,9 +226,12 @@ Section parameterized.
     intros.
     specialize (H g g').
     destruct (tac g); inv_all; subst.
-    { eapply H. reflexivity. }
+    { eapply H; eauto. }
     { forward. }
   Qed.
+
+  Variable substV : (nat -> option expr) -> expr -> expr.
+  Variable Var : nat -> expr.
 
   Definition INTRO (open : expr -> option ((typ + expr) * expr)) : rtac :=
     fun g => at_bottom (m := option)
@@ -215,6 +242,12 @@ Section parameterized.
                               match open g with
                                 | None => None
                                 | Some (inl t, g') =>
+                                  let nv := length tvs in
+                                  let g' := substV (fun v =>
+                                                      match v with
+                                                        | 0 => Some (Var nv)
+                                                        | _ => None
+                                                      end) g' in
                                   Some (GAlls t (GGoal s (Some g')))
                                 | Some (inr t, g') =>
                                   Some (GHyps t (GGoal s (Some g')))
@@ -236,13 +269,60 @@ Section parameterized.
           False
       end.
 
+  Lemma goalD_conv
+  : forall tus tvs tus' tvs' (pfu : tus' = tus) (pfv : tvs' = tvs),
+      goalD tus tvs =
+      match pfu in _ = t
+            return Goal -> option (HList.hlist _ t -> _) with
+        | eq_refl =>
+          match pfv in _ = t
+                return Goal -> option (_ -> HList.hlist _ t -> _) with
+            | eq_refl => goalD tus' tvs'
+          end
+      end.
+  Proof.
+    clear. destruct pfu; destruct pfv. reflexivity.
+  Qed.
+
+  Lemma _impls_sem
+  : forall ls P,
+      _impls ls P <-> (Forall (fun x => x) ls -> P).
+  Proof.
+    induction ls; simpl; intros.
+    + intuition.
+    + rewrite IHls. intuition.
+      inversion H0. eapply H; eauto.
+  Qed.
+  Lemma _exists_iff
+  : forall ls P Q,
+      (forall x, P x <-> Q x) ->
+      (@_exists ls P <-> @_exists ls Q).
+  Proof.
+    clear.
+    induction ls; simpl; intros.
+    + eapply H.
+    + apply exists_iff; intro. eapply IHls.
+      intro; eapply H.
+  Qed.
+  Lemma _forall_iff
+  : forall ls P Q,
+      (forall x, P x <-> Q x) ->
+      (@_foralls ls P <-> @_foralls ls Q).
+  Proof.
+    clear.
+    induction ls; simpl; intros.
+    + eapply H.
+    + apply forall_iff; intro. eapply IHls.
+      intro; eapply H.
+  Qed.
+
   Lemma at_bottom_sound_option
   : forall goal tus tvs f goal',
-      (** I need a characterization of [f] **)
       (forall tus' tvs' s e e',
          f (tus ++ tus') (tvs ++ tvs') s e = Some e' ->
+         WellFormed_subst s ->
          match goalD (tus ++ tus') (tvs ++ tvs') (GGoal s e)
-               , goalD (tus ++ tus') (tvs ++ tvs') e'
+             , goalD (tus ++ tus') (tvs ++ tvs') e'
          with
            | None , _ => True
            | Some _ , None => False
@@ -251,8 +331,9 @@ Section parameterized.
                g' us vs -> g us vs
          end) ->
       at_bottom f tus tvs goal = Some goal' ->
+      forall (Hwf : WellFormed_goal goal),
       match goalD tus tvs goal
-            , goalD tus tvs goal'
+          , goalD tus tvs goal'
       with
         | None , _ => True
         | Some _ , None => False
@@ -263,32 +344,87 @@ Section parameterized.
   Proof.
     induction goal; simpl; intros.
     { forwardy. inv_all; subst.
-      eapply IHgoal in H0.
-      simpl. forward. auto.
-      intros.
-      specialize (H tus' (t :: tvs') s e).
-      rewrite app_ass in H1. simpl in *.
-      eapply H in H1; clear H IHgoal.
-      forward.
-      destruct e.
-      admit. admit. }
-    { admit.
-    (* forwardy; inv_all; subst.
-        eapply IHgoal in H.
-        simpl; forward; eauto.
-        destruct H2. exists x.
-        eapply H1. eassumption. *) }
-    { admit.
-    (* forwardy; inv_all; subst.
-        eapply IHgoal in H.
-        simpl. forward; eauto.
-        inv_all; subst. simpl in *.
-        eauto. *) }
+      eapply IHgoal in H0; clear IHgoal; auto.
+      { simpl. forward. auto. }
+      { intros.
+        specialize (H tus' (t :: tvs') s e).
+        rewrite app_ass in H1. simpl in *.
+        eapply H in H1; clear H; auto.
+        forward.
+        rewrite substD_conv
+           with (pfu := eq_refl _) (pfv := eq_sym (HList.app_ass_trans _ _ _)) in H.
+        unfold propD in *.
+        rewrite exprD'_typ0_conv with (pfu := eq_refl _)
+             (pfv := eq_sym (HList.app_ass_trans _ _ _)) in H.
+        simpl in *.
+        unfold ResType in *.
+        autorewrite with eq_rw in *.
+        destruct e; forwardy.
+        { inv_all; subst.
+          rewrite H in *.
+          autorewrite with eq_rw in H3.
+          forwardy.
+          rewrite H3 in *.
+          inv_all; subst.
+          rewrite goalD_conv with (pfu := eq_refl)
+                                  (pfv := eq_sym (HList.app_ass_trans _ _ _)).
+          simpl.
+          forwardy.
+          autorewrite with eq_rw.
+          rewrite H1.
+          intros us vs. autorewrite with eq_rw.
+          clear - H4.
+          match goal with
+            | |- _ _ match ?X with _ => _ end ->
+                 _ _ match ?Y with _ => _ end /\
+                 _ _ match ?Z with _ => _ end =>
+              change X with Y ; change Z with Y ; destruct Y
+          end.
+          eauto. }
+        { rewrite H in *.
+          rewrite goalD_conv with (pfu := eq_refl)
+                                  (pfv := eq_sym (HList.app_ass_trans _ _ _)).
+          simpl.
+          forwardy.
+          autorewrite with eq_rw.
+          rewrite H1. intros.
+          inv_all; subst.
+          revert H6.
+          match goal with
+            | |- match ?X with _ => _ end _ _ ->
+                 match ?Y with _ => _ end _ _ =>
+              change Y with X ; destruct X
+          end. auto. } } }
+    { forwardy; inv_all; subst.
+      eapply IHgoal in H0; clear IHgoal; auto.
+      + simpl; forward; eauto.
+        destruct H3. eauto.
+      + intros.
+        rewrite goalD_conv
+           with (pfu := eq_sym (HList.app_ass_trans _ _ _))
+                (pfv := eq_refl).
+        autorewrite with eq_rw.
+        simpl. forward.
+        rewrite HList.app_ass_trans in H1.
+        simpl in H1.
+        eapply H in H1; clear H; eauto.
+        destruct e; forward.
+        - inv_all; subst.
+          revert H7. autorewrite with eq_rw.
+          eauto.
+        - inv_all; subst.
+          revert H6. autorewrite with eq_rw.
+          eauto. }
+    { forwardy; inv_all; subst.
+      eapply IHgoal in H0; clear IHgoal; eauto.
+      + simpl; forward; eauto.
+        inv_all. subst.
+        eapply _impls_sem; intro.
+        eapply _impls_sem in H5; eauto. }
     { specialize (H nil nil s o goal').
       simpl in H.
       repeat rewrite HList.app_nil_r_trans in H.
-      eapply H in H0; clear H.
-      auto. }
+      eapply H in H0; clear H; auto. }
   Qed.
 
   Theorem INTRO_sound
@@ -298,20 +434,297 @@ Section parameterized.
     unfold rtac_sound, INTRO.
     intros.
     eapply at_bottom_sound_option in H0; eauto.
-    + clear - H.
-      simpl. intros.
-      forward. inv_all; subst.
-      eapply H in H2.
-      eapply H2 in H5; clear H2.
-      destruct s0.
-      - inv_all; subst.
-        simpl.
-        (** TODO : This doesn't quite work!
-         ** The order of quantifiers is backwards
-         **)
+(*
+    { destruct (goalD nil nil g); destruct (goalD nil nil g'); auto.
+*)
   Abort.
-    
 
+  Definition STAC_no_hyps (tac : stac typ expr subst) : rtac :=
+    at_bottom (m := option)
+              (fun tus tvs sub gl =>
+                 match gl with
+                   | None => Some (GGoal sub None)
+                   | Some gl =>
+                     match tac tus tvs sub nil gl with
+                       | Fail => None
+                       | More tus' tvs' sub' hs' gl' =>
+                         ret (List.fold_right GExs
+                               (List.fold_right GAlls
+                                 (List.fold_right GHyps
+                                   (GGoal sub' (Some gl')) hs') tvs') tus')
+                       | Solved tus' tvs' sub' =>
+                         ret (List.fold_right GExs
+                               (List.fold_right GAlls
+                                 (GGoal sub' None) tvs') tus')
+                     end
+                 end)
+              nil nil.
+
+  Lemma goalD_fold_right_GExs
+  : forall tvs g ls tus,
+      match goalD tus tvs (fold_right GExs g ls)
+          , goalD (tus ++ ls) tvs g
+      with
+        | Some D , Some D' =>
+          forall us vs,
+            D us vs <->
+            _exists
+              (fun us' : HList.hlist (typD nil) ls =>
+                 D' (HList.hlist_app us us') vs)
+        | None , None => True
+        | _ , _ => False
+      end.
+  Proof.
+    clear.
+    induction ls; simpl.
+    { intros.
+      rewrite goalD_conv
+      with (pfu := eq_sym (HList.app_nil_r_trans _)) (pfv := eq_refl).
+      autorewrite with eq_rw.
+      destruct (goalD tus tvs g); auto.
+      intros. rewrite HList.hlist_app_nil_r.
+      clear.
+      match goal with
+        | |- _ <-> (match ?X with _ => _ end
+                      match ?Y with _ => _ end _) =>
+          change Y with X ; destruct X
+      end.
+      reflexivity. }
+    { intros.
+      specialize (IHls (tus ++ a :: nil)).
+      rewrite goalD_conv
+      with (pfu := eq_sym (HList.app_ass_trans _ _ _)) (pfv := eq_refl)
+        in IHls.
+      autorewrite with eq_rw in IHls. simpl in *.
+      destruct (goalD (tus ++ a :: nil) tvs (fold_right GExs g ls));
+        destruct (goalD (tus ++ a :: ls) tvs g); auto.
+      intros.
+      eapply exists_iff; intro.
+      etransitivity. eapply IHls.
+      eapply _exists_iff; intro.
+      autorewrite with eq_rw.
+      match goal with
+        | |- ?X <-> ?Y =>
+          cutrewrite (X = Y); try reflexivity
+      end.
+      f_equal.
+      clear.
+      change (HList.Hcons x x0)
+      with (HList.hlist_app (HList.Hcons x HList.Hnil) x0).
+      rewrite HList.hlist_app_assoc.
+      simpl.
+      apply Eq.match_eq_sym_eq'. }
+  Qed.
+
+  Lemma goalD_fold_right_GAlls
+  : forall tus g ls tvs,
+      match goalD tus tvs (fold_right GAlls g ls)
+          , goalD tus (tvs ++ ls) g
+      with
+        | Some D , Some D' =>
+          forall us vs,
+            D us vs <->
+            _foralls
+              (fun vs' : HList.hlist (typD nil) ls =>
+                 D' us (HList.hlist_app vs vs'))
+        | None , None => True
+        | _ , _ => False
+      end.
+  Proof.
+    clear.
+    induction ls; simpl.
+    { intros.
+      rewrite goalD_conv
+      with (pfu := eq_refl) (pfv := eq_sym (HList.app_nil_r_trans _)).
+      autorewrite with eq_rw.
+      destruct (goalD tus tvs g); auto.
+      intros. rewrite HList.hlist_app_nil_r.
+      clear.
+      match goal with
+        | |- _ <-> (match ?X with _ => _ end
+                      _ match ?Y with _ => _ end) =>
+          change Y with X ; destruct X
+      end.
+      reflexivity. }
+    { intros.
+      specialize (IHls (tvs ++ a :: nil)).
+      rewrite goalD_conv
+      with (pfu := eq_refl) (pfv := eq_sym (HList.app_ass_trans _ _ _))
+        in IHls.
+      autorewrite with eq_rw in IHls. simpl in *.
+      destruct (goalD tus (tvs ++ a :: nil) (fold_right GAlls g ls));
+        destruct (goalD tus (tvs ++ a :: ls) g); auto.
+      intros.
+      eapply forall_iff; intro.
+      etransitivity. eapply IHls.
+      eapply _forall_iff; intro.
+      autorewrite with eq_rw.
+      match goal with
+        | |- ?X <-> ?Y =>
+          cutrewrite (X = Y); try reflexivity
+      end.
+      f_equal.
+      clear.
+      change (HList.Hcons x x0)
+      with (HList.hlist_app (HList.Hcons x HList.Hnil) x0).
+      rewrite HList.hlist_app_assoc.
+      simpl.
+      apply Eq.match_eq_sym_eq'. }
+  Qed.
+
+  Lemma _exists_sem : forall ls P,
+                        _exists (ls := ls) P <->
+                        exists x, P x.
+  Proof.
+    clear. induction ls; simpl; auto.
+    - intuition. exists HList.Hnil. auto.
+      destruct H. rewrite (HList.hlist_eta x) in H.
+      assumption.
+    - intros. split.
+      + destruct 1.
+        eapply IHls in H.
+        destruct H. eauto.
+      + destruct 1.
+        exists (HList.hlist_hd x).
+        eapply IHls.
+        exists (HList.hlist_tl x).
+        rewrite (HList.hlist_eta x) in H.
+        assumption.
+  Qed.
+  Lemma _forall_sem : forall ls P,
+                        _foralls (ls := ls) P <->
+                        forall x, P x.
+  Proof.
+    clear. induction ls; simpl; auto.
+    - intuition. rewrite (HList.hlist_eta x).
+      assumption.
+    - intros. split.
+      + intros.
+        rewrite (HList.hlist_eta x).
+        eapply IHls in H.
+        eapply H.
+      + intros.
+        eapply IHls.
+        intros. eapply H.
+  Qed.
+
+  Lemma at_bottom_WF_option
+  : forall f,
+      (forall a b c d g,
+         f a b c d = Some g ->
+         WellFormed_subst c ->
+         WellFormed_goal g) ->
+    forall g tus tvs g',
+      at_bottom f tus tvs g = Some g' ->
+      WellFormed_goal g ->
+      WellFormed_goal g'.
+  Proof.
+    clear.
+    induction g; simpl; intros; forwardy; inv_all; subst; simpl in *; eauto.
+  Qed.
+
+  Lemma WellFormed_goal_GAlls
+  : forall ls g,
+      WellFormed_goal g <-> WellFormed_goal (fold_right GAlls g ls).
+  Proof.
+    clear. induction ls; simpl; intros; auto.
+    reflexivity.
+  Qed.
+  Lemma WellFormed_goal_GExs
+  : forall ls g,
+      WellFormed_goal g <-> WellFormed_goal (fold_right GExs g ls).
+  Proof.
+    clear. induction ls; simpl; intros; auto.
+    reflexivity.
+  Qed.
+  Lemma WellFormed_goal_GHyps
+  : forall ls g,
+      WellFormed_goal g <-> WellFormed_goal (fold_right GHyps g ls).
+  Proof.
+    clear. induction ls; simpl; intros; auto.
+    reflexivity.
+  Qed.
+
+
+  Theorem STAC_no_hyps_sound
+  : forall tac, stac_sound tac ->
+                rtac_sound nil nil (STAC_no_hyps tac).
+  Proof.
+(*
+    intros.
+    unfold rtac_sound, STAC_no_hyps.
+    intros. split.
+    { eapply at_bottom_WF_option in H0; auto.
+      destruct d.
+      + intros. specialize (H a b c nil e H3).
+        destruct (tac a b c nil e); try congruence.
+        - destruct H. clear - H H2.
+          inversion H2.
+          apply WellFormed_goal_GExs.
+          apply WellFormed_goal_GAlls.
+          simpl. assumption.
+        - destruct H; clear - H H2.
+          inversion H2.
+          apply WellFormed_goal_GExs.
+          apply WellFormed_goal_GAlls.
+          apply WellFormed_goal_GHyps.
+          simpl. assumption.
+      + clear. inversion 1.
+        refine (fun x => x). }
+    eapply at_bottom_sound_option in H0; eauto; clear H0.
+    simpl.
+    intros.
+    destruct e.
+    { assert (WellFormed_subst s) by admit.
+      consider (tac tus' tvs' s nil e); try congruence;
+      intros; inv_all; subst.
+      { specialize (H tus' tvs' s nil e H1).
+        rewrite H0 in H; clear H0 H1.
+        forward_reason.
+        unfold stateD in *.
+        unfold propD, Core.propD in *.
+        forward.
+        simpl in H2.
+        forwardy.
+        specialize (goalD_fold_right_GExs tvs'
+                      (fold_right GAlls (GGoal s0 None) l0)
+                      l tus').
+        match goal with
+          | |- match ?X with _ => _ end ->
+               match ?Y with _ => _ end =>
+            change Y with X ; destruct X
+        end;
+        specialize (goalD_fold_right_GAlls (tus' ++ l)
+                      (GGoal s0 None)
+                      l0 tvs');
+        match goal with
+          | |- match ?X with _ => _ end ->
+               match ?Y with _ => _ end -> _ =>
+            change Y with X ; destruct X
+        end; auto.
+        { simpl. intros; forwardy.
+          inv_all; subst.
+          eapply H3; auto; clear H3.
+          eapply H5 in H6; clear H5.
+          eapply _exists_sem in H6.
+          destruct H6.
+          exists x.
+          intros.
+          change_rewrite H2 in H4.
+          inv_all; subst.
+          eapply H7 in H3; clear H7.
+          eapply _forall_sem in H3. eapply H3. }
+        { inversion 2. }
+        { simpl. rewrite H2. auto. } }
+      { specialize (H tus' tvs' s nil e H1).
+        rewrite H0 in H.
+        
+
+ } }
+    { inv_all; subst.
+      simpl. forward. }
+*)
+  Abort.
 
   Eval compute in fun open t1 t2 e3 s goal =>
     INTRO open (GAlls t1 (GExs t2 (GHyps e3 (GGoal s (Some goal))))).
