examples/RTac/Demo.v
@@ -1,0 +1,81 @@
+Require Import ExtLib.Core.RelDec.
+Require Import MirrorCore.Lambda.ExprCore.
+Require Import MirrorCore.Lambda.Red.
+Require Import McExamples.Simple.Simple.
+Require Import MirrorCore.RTac.CoreSimple.
+
+Definition simple_goal : expr typ func :=
+  App (Inj (All tyProp)) (Abs tyProp (App (App (Inj Impl) (Var 0)) (Var 0))).
+
+Definition open (e : expr typ func)
+: option ((typ + expr typ func) * expr typ func) :=
+  match e with
+    | App (Inj (All t)) e =>
+      Some (inl t, beta (App e (Var 0)))
+    | App (App (Inj Impl) P) Q =>
+      Some (inr P, Q)
+    | _ => None
+  end.
+
+Inductive Ctx :=
+| CTop
+| CAll : typ -> Ctx -> Ctx
+| CEx  : typ -> Ctx -> Ctx
+| CHyp : expr typ func -> Ctx -> Ctx.
+
+Fixpoint openGoal' {subst} (g : Goal typ (expr typ func) subst) (ctx : Ctx)
+: Ctx * subst * option (expr typ func) :=
+  match g with
+    | GGoal s e => (ctx,s,e)
+    | GAlls t g => openGoal' g (CAll t ctx)
+    | GExs  t g => openGoal' g (CEx  t ctx)
+    | GHyps h g => openGoal' g (CHyp h ctx)
+  end.
+
+Definition openGoal {subst} g := @openGoal' subst g CTop.
+
+Fixpoint closeGoal {subst} (ctx : Ctx) (g : Goal typ (expr typ func) subst)
+: Goal typ (expr typ func) subst :=
+  match ctx with
+    | CTop => g
+    | CAll t c => closeGoal c (GAlls t g)
+    | CEx t c => closeGoal c (GExs t g)
+    | CHyp t c => closeGoal c (GHyps t g)
+  end.
+
+Section assumption.
+  Context {subst : Type}.
+  Variable (check : expr typ func -> expr typ func -> subst -> option subst).
+
+  Fixpoint findHyp s (ctx : Ctx) (g : expr typ func) {struct ctx}
+  : option subst :=
+    match ctx with
+      | CTop => None
+      | CAll t ctx' => findHyp s ctx' g
+      | CEx  t ctx' => findHyp s ctx' g
+      | CHyp h ctx' => match check g h s with
+                         | None => findHyp s ctx' g
+                         | Some e => Some e
+                       end
+    end.
+
+  Definition ASSUMPTION : rtac typ (expr typ func) subst :=
+    fun g =>
+      let '(ctx,s,gl) := openGoal g in
+      match gl with
+        | None => Some g
+        | Some gl => match findHyp s ctx gl with
+                       | None => None
+                       | Some s => Some (@closeGoal _ ctx (GGoal _ s None))
+                     end
+      end.
+End assumption.
+
+Let INTRO {subst} :=
+  INTRO (subst:=subst) (fun f e => substitute_all f 0 e) (@Var typ func) open.
+
+Definition tac subst : rtac typ (expr typ func) subst :=
+  THEN INTRO (THEN INTRO (ASSUMPTION (fun x y s => if x ?[ eq ] y then Some s else None))).
+
+Eval compute in fun subst (empty : subst) =>
+                  tac subst (@GGoal _ _ _ empty (Some simple_goal)).
