theories/RTac/Core.v
@@ -552,3 +552,4 @@ remember (rev (tvs ++ rev (t :: l))).
       exists x0. apply H. auto. }
   Qed.
 *)
+End parameterized.
